@prefix dc:      <http://purl.org/dc/elements/1.1/> .
@prefix dct:     <http://purl.org/dc/terms/> .
@prefix owl:     <http://www.w3.org/2002/07/owl#> .
@prefix org:     <http://www.w3.org/ns/org#> .
@prefix odrl:    <http://www.w3.org/ns/odrl/2/> .
@prefix profile: <http://www.w3.org/ns/dx/prof/> .
@prefix rdfs:    <http://www.w3.org/2000/01/rdf-schema#> .
@prefix role:    <http://www.w3.org/ns/dx/prof/role/> .
@prefix skos:    <http://www.w3.org/2004/02/skos/core#> .
@prefix vann:    <http://purl.org/vocab/vann/> .
@prefix voaf:    <http://purl.org/vocommons/voaf#> .
@prefix void:    <http://rdfs.org/ns/void#> .
@prefix xsd:     <http://www.w3.org/2001/XMLSchema#> .

@prefix EU:      <https://european-union.europa.eu/> .

@prefix lds:     <https://github.com/nicosResearchAndDevelopment/LDS/> .
@prefix entity:  <https://github.com/nicosResearchAndDevelopment/LDS/model/concept/higher/entity/> .
@prefix nis2:    <https://github.com/nicosResearchAndDevelopment/NIS2/> .

<https://github.com/nicosResearchAndDevelopment/NIS2/>
    a                             voaf:Vocabulary ;
    a                             owl:Ontology ;
    skos:prefLabel                "European Network and Information Security legislation, NIS2"^^xsd:string ;
    rdfs:label                    "European Network and Information Security legislation, NIS2"@en ;
    dct:title                     "Model for NIS2"@en ;
    dct:description               """"""@en ;
## TODO : cc:license                    <> ;
    dct:creator                   <https://jlangkau.solidweb.org/> ;
    dct:publisher                 <https://www.nicos-ag.com> ;
    dct:created                   "2023-02-19"^^xsd:date ;
    ## TODO: dct:modified                  {{now.date}} ;
    owl:versionInfo               "1.0.0" ;
    ## TODO: owl:versionInfo               {{version.ontology}} ;
    vann:preferredNamespaceUri    "https://github.com/nicosResearchAndDevelopment/NIS2/"^^xsd:anyURI ;
    vann:preferredNamespacePrefix "nis2:" ;
    void:vocabulary               vann:, void:, voaf:, dct: ;
    ####################################################################################################################
    skos:broader                  EU:DIRECTIVE_2018-1972 ; # <<<<<<<<<<<<<<<<<<<<<<<<<<<<<<<<<<<<<<<<<<<<<<<<<<<<<<<<<<<
    ####################################################################################################################
    rdfs:seeAlso                  <https://github.com/nicosResearchAndDevelopment/NIS2/> ;
    rdfs:isDefinedBy              <https://jlangkau.solidweb.org/> .

## region Article

nis2:Article
    ## TODO: abstract
    a                owl:Class ;
    skos:notation    "Article"^^xsd:string ;
    skos:prefLabel   "Article"^^xsd:string ;
    rdfs:label       "Article"@en ;
    rdfs:label       "Artikel"@de ;
    rdfs:isDefinedBy nis2: .

nis2:article
    a                owl:ObjectProperty ;
    rdfs:label       "Article"@en ;
    rdfs:label       "Artikel"@de ;
    skos:notation    "Article"^^xsd:string ;
    skos:prefLabel   "Article"^^xsd:string ;
    rdfs:domain      nis2:Compliance ;
    rdfs:range       nis2:Article ;
    rdfs:isDefinedBy nis2: .

## region Article Individuals

nis2:Article-10
    a                skos:Concept, nis2:Article ;
    rdfs:label       "Article 10"@en ;
    rdfs:label       "Artikel 10"@de ;
    dct:description  "Computer security incident response teams (CSIRTs)"@en ;
    nis2:compliant   nis2:Article-10-Compliance ;
    skos:notation    "Article-10"^^xsd:string ;
    skos:prefLabel   "Article 10"^^xsd:string ;
    rdfs:isDefinedBy nis2: .

## endregion Article Individuals

## endregion Article

## region Compliance

nis2:Compliance
    ## TODO: abstract
    a                owl:Class ;
    rdfs:label       "Compliance"@en ;
    rdfs:label       "Regelkonformität"@de ;
    skos:notation    "Compliance"^^xsd:string ;
    skos:prefLabel   "Compliance"^^xsd:string ;
    skos:narrower    nis2:Article-10-Compliance ;
    rdfs:isDefinedBy nis2: .

nis2:compliant
    a                owl:ObjectProperty ;
    rdfs:label       "Compliant"@en ;
    rdfs:label       "Regelkonform"@de ;
    skos:notation    "compliant"^^xsd:string ;
    skos:prefLabel   "Compliant"^^xsd:string ;
    rdfs:domain      nis2:Article ;
    rdfs:domain      nis2:Agent ;
    rdfs:range       nis2:Compliance ;
    rdfs:isDefinedBy nis2: .

## region Compliance Individuals
## region Compliance Individuals "Article 10"

nis2:Article-10-Compliance
    a                skos:Concept, nis2:Compliance ;
    rdfs:label       "Article 10 Compliance"@en ;
    rdfs:label       "Artikel 10 Regelkonformität"@de ;
    nis2:article     nis2:Article-10 ;
    skos:notation    "Article-10-Compliance"^^xsd:string ;
    skos:prefLabel   "Article 10 Compliance"^^xsd:string ;
    skos:broader     nis2:Compliance ;
    skos:related     nis2:Article-10 ;
    rdfs:isDefinedBy nis2: .

nis2:Article-10-MemberState-Compliance
    a                skos:Concept, nis2:Compliance ;
    rdfs:label       """Article 10 "Member State" Compliance"""@en ;
    rdfs:label       """Artikel 10 "Mitgliedstaat"-Regelkonformität"""@de ;
    nis2:article     nis2:Article-10 ;
    skos:notation    "Article-10-MemberState-Compliance"^^xsd:string ;
    skos:prefLabel   """Article 10 "Member State" Compliance"""^^xsd:string ;
    skos:broader     nis2:Article-10-Compliance ;
    skos:related     nis2:Article-10 ;
    skos:related     nis2:MemberState ;
    rdfs:isDefinedBy nis2: .

nis2:Article-10-CSIRT-Compliance
    a                skos:Concept, nis2:Compliance ;
    rdfs:label       """Article 10 "CSIRT" Compliance"""@en ;
    rdfs:label       """Artikel 10 "CSIRT"-Regelkonformität"""@de ;
    nis2:article     nis2:Article-10 ;
    skos:notation    "Article-10-CSIRT-Compliance"^^xsd:string ;
    skos:prefLabel   """Article 10 "CSIRT" Compliance"""^^xsd:string ;
    skos:broader     nis2:Article-10-Compliance ;
    skos:related     nis2:Article-10 ;
    skos:related     nis2:CSIRT ;
    rdfs:isDefinedBy nis2: .

## endregion Compliance Individuals "Article 10"
## endregion Compliance Individuals

## endregion Compliance

## region Criticality

nis2:Criticality
    a                owl:Class ;
    rdfs:label       "Criticality"@en ;
    rdfs:label       "Kritikalität"@en ;
    skos:notation    "Criticality"^^xsd:string ;
    skos:prefLabel   "Criticality"^^xsd:string ;
    skos:narrower    nis2:Criticality_HIGH ;
    skos:narrower    nis2:Criticality_MID ;
    skos:narrower    nis2:Criticality_LOW ;
    skos:narrower    nis2:Criticality_OTHER ;
    rdfs:isDefinedBy nis2: .

nis2:criticality
    a                owl:ObjectProperty ;
    rdfs:label       "Criticality"@en ;
    rdfs:label       "Kritikalität"@de ;
    skos:notation    "criticality"^^xsd:string ;
    skos:prefLabel   "Criticality"^^xsd:string ;
    rdfs:range       nis2:Criticality ;
    rdfs:isDefinedBy nis2: .

## region Criticality Individuals

nis2:Criticality_HIGH
    a                nis2:Criticality, owl:NamedIndividual ;
    rdfs:label       "High criticality"@en ;
    rdfs:label       "Hohe Kritikalität"@de ;
    skos:notation    "Criticality_HIGH"^^xsd:string ;
    skos:prefLabel   "High criticality"^^xsd:string ;
    skos:broader     nis2:Criticality ;
    skos:related     nis2:Criticality_OTHER ;
    rdfs:comment     """See also ("ANNEX I, SECTORS OF HIGH CRITICALITY"): <https://eur-lex.europa.eu/legal-content/EN/TXT/HTML/?uri=CELEX:32022L2555#d1e32-143-1>."""@en ;
    rdfs:seeAlso     <https://eur-lex.europa.eu/legal-content/EN/TXT/HTML/?uri=CELEX:32022L2555#d1e32-143-1> ;
    rdfs:isDefinedBy nis2: .

nis2:Criticality_OTHER
    a                nis2:Criticality, owl:NamedIndividual ;
    rdfs:label       "Other criticality"@en ;
    rdfs:label       "Weitere Kritikalität"@de ;
    skos:notation    "Criticality_OTHER"^^xsd:string ;
    skos:prefLabel   "Other criticality"^^xsd:string ;
    skos:broader     nis2:Criticality ;
    skos:related     nis2:Criticality_HIGH ;
    rdfs:comment     """See also ("ANNEX II, OTHER CRITICAL SECTORS"): <https://eur-lex.europa.eu/legal-content/EN/TXT/HTML/?uri=CELEX:32022L2555#d1e32-148-1>."""@en ;
    rdfs:seeAlso     <https://eur-lex.europa.eu/legal-content/EN/TXT/HTML/?uri=CELEX:32022L2555#d1e32-148-1> ;
    rdfs:isDefinedBy nis2: .

## endregion Criticality Individuals

## endregion Criticaity

## region Actor

nis2:Actor
    ## TODO: abstract
    a                owl:Class ;
    rdfs:label       "Actor"@en ;
    rdfs:label       "Akteur"@de ;
    skos:notation    "Actor"^^xsd:string ;
    skos:prefLabel   "Actor"^^xsd:string ;
    rdfs:isDefinedBy nis2: .

## region Actor Agent

nis2:Agent
    ## TODO: TBSD: !!!! abstract ??????????????
    a                owl:Class ;
    rdfs:subClassOf  nis2:Actor ;
    rdfs:label       "Agent"@en ;
    rdfs:label       "Agent"@de ;
    skos:notation    "Agent"^^xsd:string ;
    skos:prefLabel   "Agent"^^xsd:string ;
    rdfs:comment     """So, instances of 'nis2:Actor' are Participants of given Eco-System or Data Space..."""@en ;
    rdfs:isDefinedBy nis2: .

nis2:agent
    a                owl:ObjectProperty ;
    rdfs:label       "Agent"@en ;
    rdfs:label       "Agent"@de ;
    skos:notation    "agent"^^xsd:string ;
    skos:prefLabel   "Agent"^^xsd:string ;
## TODO: TBD:    rdfs:domain      ;
    rdfs:range       nis2:Agent ;
    rdfs:isDefinedBy nis2: .

@prefix foaf: <http://xmlns.com/foaf/0.1/> .

nis2:CSIRT
    a                owl:Class ;
    rdfs:subClassOf  nis2:Agent ;
    rdfs:label       "CSIRT"@en ;
    rdfs:label       "CSIRT"@de ;
    skos:notation    "CSIRT"^^xsd:string ;
    skos:prefLabel   "CSIRT"^^xsd:string ;
    rdfs:isDefinedBy nis2: .

## region Actor Agent Institution

nis2:Institution
    ## TODO: abstract
    ## TODO: TBD: ...or nis2:Authority
    a                owl:Class ;
    rdfs:subClassOf  nis2:Agent ;
    rdfs:label       "Institution"@en ;
    rdfs:label       "Institution"@de ;
    skos:notation    "Institution"^^xsd:string ;
    skos:prefLabel   "Institution"^^xsd:string ;
    rdfs:isDefinedBy nis2: .

nis2:MemberState
    a                owl:Class ;
    rdfs:subClassOf  nis2:Institution ;
    rdfs:subClassOf  nis2:Agent ;
    rdfs:label       "Member state"@en ;
    rdfs:label       "Mitgliedstaat"@de ;
    skos:notation    "MemberState"^^xsd:string ;
    skos:prefLabel   "Member State"^^xsd:string ;
    rdfs:isDefinedBy nis2: .

nis2:Representative
    a                owl:Class ;
    rdfs:subClassOf  nis2:Institution ;
    rdfs:subClassOf  nis2:Agent ;
    rdfs:label       "Representative"@en ;
    rdfs:label       "Repräsentant"@de ;
    skos:notation    "Representative"^^xsd:string ;
    skos:prefLabel   "Representative"^^xsd:string ;
    rdfs:isDefinedBy nis2: .

## endregion Actor Agent Institution
## endregion Actor Agent

## endregion Actor

## region Sector

nis2:Sector
    a                owl:Class ;
    rdfs:label       "Sector"@en ;
    rdfs:label       "Sektor"@de ;
    skos:notation    "Sector"^^xsd:string ;
    skos:prefLabel   "Sector"^^xsd:string ;
    rdfs:isDefinedBy nis2: .

nis2:sector
    a                owl:ObjectProperty ;
    rdfs:label       "Sector"@en ;
    rdfs:label       "Sector"@de ;
    skos:notation    "sector"^^xsd:string ;
    skos:prefLabel   "Sector"^^xsd:string ;
## TODO: TBD:    rdfs:domain      ;
    rdfs:range       nis2:Sector ;
    rdfs:isDefinedBy nis2: .

nis2:SubSector
    a                owl:Class ;
    rdfs:subClassOf  nis2:Sector ;
    rdfs:label       "Sub-sector"@en ;
    rdfs:label       "Sub-Sektor"@de ;
    skos:notation    "SubSector"^^xsd:string ;
    skos:prefLabel   "SubSector"^^xsd:string ;
    rdfs:isDefinedBy nis2: .

nis2:subSector
    a                owl:ObjectProperty ;
    owl:inverseOf    nis2:subSectorOf ;
    rdfs:label       "Sub-sector"@en ;
    rdfs:label       "Sub-Sektor"@de ;
    skos:notation    "subSector"^^xsd:string ;
    skos:prefLabel   "subSector"^^xsd:string ;
    rdfs:domain      nis2:Sector ;
    rdfs:range       nis2:SubSector ;
    rdfs:isDefinedBy nis2: .

nis2:subSectorOf
    a                owl:ObjectProperty ;
    owl:inverseOf    nis2:subSector ;
    rdfs:label       "Sub-sector of"@en ;
    rdfs:label       "Sub-Sektor von"@de ;
    skos:notation    "subSectorOf"^^xsd:string ;
    skos:prefLabel   "subSectorOf"^^xsd:string ;
    rdfs:domain      nis2:SubSector ;
    rdfs:range       nis2:SubSector ;   ## REM: even NIS2 Directive shows no Sub-sectors of Sub-sectors we put in here...
    rdfs:range       nis2:Sector ;
    rdfs:isDefinedBy nis2: .

## endregion Sector

## Sector Individuals

nis2:Energy_Sector
    a                nis2:Sector, owl:NamedIndividual ;
    rdfs:label       "Energy Sector"@en ;
    rdfs:label       "Energie Sektor"@de ;
    skos:notation    "Energy_Sector"^^xsd:string ;
    skos:prefLabel   "Energy Sector"^^xsd:string ;
    nis2:criticality nis2:Criticality_HIGH ;
    nis2:subSector   nis2:Energy-Electricity_Sector ;
    nis2:subSector   nis2:Energy-DistrictHeatingAndCooling_Sector ;
    skos:narrower    nis2:Energy-Electricity_Sector ;
    skos:narrower    nis2:Energy-DistrictHeatingAndCooling_Sector ;
    rdfs:seeAlso     <https://eur-lex.europa.eu/legal-content/EN/TXT/HTML/?uri=CELEX:32022L2555#d1e32-143-1> ;
    rdfs:isDefinedBy nis2: .

nis2:Energy-Electricity_Sector
    a                nis2:SubSector, owl:NamedIndividual ;
    rdfs:label       "Electricity Sector (Energy)"@en ;
    rdfs:label       "Elektrizität-Sector (Energy)"@de ;
    dct:description  """- Electricity undertakings as defined in Article 2, point (57), of Directive (EU) 2019/944 of the European Parliament and of the Council (1), which carry out the function of ‘supply’ as defined in Article 2, point (12), of that Directive
- Distribution system operators as defined in Article 2, point (29), of Directive (EU) 2019/944
- Transmission system operators as defined in Article 2, point (35), of Directive (EU) 2019/944
- Producers as defined in Article 2, point (38), of Directive (EU) 2019/944
- Nominated electricity market operators as defined in Article 2, point (8), of Regulation (EU) 2019/943 of the European Parliament and of the Council (2)
- Market participants as defined in Article 2, point (25), of Regulation (EU) 2019/943 providing aggregation, demand response or energy storage services as defined in Article 2, points (18), (20) and (59), of Directive (EU) 2019/944
- Operators of a recharging point that are responsible for the management and operation of a recharging point, which provides a recharging service to end users, including in the name and on behalf of a mobility service provider"""@en ;
    skos:notation    "Energy-Electricity_Sector"^^xsd:string ;
    skos:prefLabel   "Energy-Electricity Sector"^^xsd:string ;
    nis2:criticality nis2:Criticality_HIGH ;
    nis2:sector      nis2:Energy_Sector ;
    skos:broader     nis2:Energy_Sector ;
    rdfs:seeAlso     <https://eur-lex.europa.eu/legal-content/EN/TXT/HTML/?uri=CELEX:32022L2555#d1e32-143-1> ;
    rdfs:isDefinedBy nis2: .

nis2:Energy-DistrictHeatingAndCooling_Sector
    a                nis2:SubSector, owl:NamedIndividual ;
    rdfs:label       "District Heating and Cooling Sector (Energy)"@en ;
    dct:description  """- Operators of district heating or district cooling as defined in Article 2, point (19), of Directive (EU) 2018/2001 of the European Parliament and of the Council (3)"""@en ;
    skos:notation    "Energy-DistrictHeatingAndCooling_Sector"^^xsd:string ;
    skos:prefLabel   "District Heating and Cooling Sector (Energy)"^^xsd:string ;
    nis2:criticality nis2:Criticality_HIGH ;
    nis2:subSectorOf nis2:Energy_Sector ;
    skos:broader     nis2:Energy_Sector ;
    rdfs:seeAlso     <https://eur-lex.europa.eu/legal-content/EN/TXT/HTML/?uri=CELEX:32022L2555#d1e32-143-1> ;
    rdfs:isDefinedBy nis2: .

nis2:Transport_Sector
    a                nis2:Sector, owl:NamedIndividual ;
    rdfs:label       "Transport Sector"@en ;
    skos:notation    "Transport_Sector"^^xsd:string ;
    skos:prefLabel   "Transport Sector"^^xsd:string ;
    nis2:criticality nis2:Criticality_HIGH ;
    nis2:subSector   nis2:Transport-Air_Sector ;
    skos:narrower    nis2:Transport-Air_Sector ;
    rdfs:seeAlso     <https://eur-lex.europa.eu/legal-content/EN/TXT/HTML/?uri=CELEX:32022L2555#d1e32-143-1> ;
    rdfs:isDefinedBy nis2: .

nis2:Transport-Air_Sector
    a                nis2:SubSector, owl:NamedIndividual ;
    rdfs:label       "Air Sector (Transport)"@en ;
    dct:description  """- Air carriers as defined in Article 3, point (4), of Regulation (EC) No 300/2008 used for commercial purposes
- Airport managing bodies as defined in Article 2, point (2), of Directive 2009/12/EC of the European Parliament and of the Council (6), airports as defined in Article 2, point (1), of that Directive, including the core airports listed in Section 2 of Annex II to Regulation (EU) No 1315/2013 of the European Parliament and of the Council (7), and entities operating ancillary installations contained within airports
- Traffic management control operators providing air traffic control (ATC) services as defined in Article 2, point (1), of Regulation (EC) No 549/2004 of the European Parliament and of the Council (8)"""@en ;
    skos:notation    "Transport-Air_Sector"^^xsd:string ;
    skos:prefLabel   "Air Sector (Transport)"^^xsd:string ;
    nis2:criticality nis2:Criticality_HIGH ;
    nis2:subSectorOf nis2:Transport_Sector ;
    skos:broader     nis2:Transport_Sector ;
    rdfs:seeAlso     <https://eur-lex.europa.eu/legal-content/EN/TXT/HTML/?uri=CELEX:32022L2555#d1e32-143-1> ;
    rdfs:isDefinedBy nis2: .

## ANNEX II, OTHER CRITICAL SECTORS

nis2:Manufacturing_Sector
    a                nis2:Sector, owl:NamedIndividual ;
    rdfs:label       "Manufacturing Sector"@en ;
    skos:notation    "Manufacturing_Sector"^^xsd:string ;
    skos:prefLabel   "Manufacturing Sector"^^xsd:string ;
    nis2:criticality nis2:Criticality_OTHER ;
    skos:narrower    nis2:Manufacturing-ElectricalEquipment_Sector ;
    rdfs:comment     """ANNEX II, OTHER CRITICAL SECTORS"""@en ;
    rdfs:seeAlso     <https://eur-lex.europa.eu/legal-content/EN/TXT/HTML/?uri=CELEX:32022L2555#d1e32-148-1> ;
    rdfs:isDefinedBy nis2: .

nis2:Manufacturing-ElectricalEquipment_Sector
    a                nis2:SubSector, owl:NamedIndividual ;
    rdfs:label       "Air Sector (Manufacturing)"@en ;
    dct:description  """Manufacture of electrical equipment"""@en ;
    skos:notation    "Manufacturing-ElectricalEquipment_Sector"^^xsd:string ;
    skos:prefLabel   "ElectricalEquipment_Sector Sector (Transport)"^^xsd:string ;
    nis2:criticality nis2:Criticality_HIGH ;
    nis2:subSectorOf nis2:Manufacturing_Sector ;
    skos:broader     nis2:Manufacturing_Sector ;
    rdfs:comment     """ANNEX II, OTHER CRITICAL SECTORS"""@en ;
    rdfs:seeAlso     <https://eur-lex.europa.eu/legal-content/EN/TXT/HTML/?uri=CELEX:32022L2555#d1e32-148-1> ;
    rdfs:isDefinedBy nis2: .